Strengthen pf_consistent_super_strong

src/prop/PFConsistentStrong.v
@@ -266,6 +266,87 @@ Qed.
 
 
 
+Definition certification_times (times : Loc.t -> list Time.t)
+           (f: Loc.t -> nat -> (Time.t -> Time.t -> Prop))
+           (max: TimeMap.t)
+           (loc: Loc.t) (fts: Time.t): Prop :=
+  ((<<IN: List.In fts (times loc)>>) /\ (<<TS: Time.le fts (max loc)>>)) \/
+  (exists ts n,
+      (<<IN: List.In ts (times loc)>>) /\ (<<TS: Time.lt (max loc) ts>>)
+      /\ (<<MAX: Time.lt (max loc) (incr_time_seq n)>>)
+      /\ (<<MAP: f loc n ts fts>>)).
+
+Lemma certification_times_well_ordered times f max
+      (MAP: forall loc n
+                   (TS: Time.lt (max loc) (incr_time_seq n)),
+          cap_flex_map_loc
+            (max loc)
+            (Time.incr (max loc))
+            (incr_time_seq n) (times loc) (f loc n))
+  :
+    forall loc, well_ordered (certification_times times f max loc).
+Proof.
+  i. hexploit (@increasing_join_well_ordered
+                 incr_time_seq
+                 (fun n fts =>
+                    (exists ts,
+                        (<<IN: List.In ts (times loc)>>) /\ (<<TS: Time.lt (max loc) ts>>)
+                        /\ (<<MAX: Time.lt (max loc) (incr_time_seq n)>>)
+                        /\ (<<MAP: f loc n ts fts>>)))).
+  { i. eapply incr_time_seq_lt; eauto. }
+  { eapply incr_time_seq_diverge. }
+  { i. des. exploit MAP; eauto. intros FLEXMAP.
+    eapply (FLEXMAP.(cap_flex_map_loc_bound)); try apply MAP0. auto. }
+  { i. assert (INJ: forall (TS: Time.lt (max loc) (incr_time_seq n))
+                           ts fts0 fts1
+                           (MAP0: f loc n ts fts0)
+                           (MAP1: f loc n ts fts1),
+                  fts0 = fts1).
+    { i. specialize (MAP _ _ TS). eapply mapping_map_lt_loc_map_eq; eauto. eapply MAP. }
+    remember (times loc). clear MAP times Heql. induction l.
+    { eapply sub_well_ordered with (times0 := bot1).
+      { eapply empty_well_ordered. }
+      { i. des. ss. }
+    }
+    { destruct (classic (exists fts,
+                            (<<TS: Time.lt (max loc) a>>)
+                            /\ (<<MAX: Time.lt (max loc) (incr_time_seq n)>>)
+                            /\ (<<MAP: f loc n a fts>>))).
+      { des. eapply sub_well_ordered.
+        { eapply join_well_ordered.
+          { eapply IHl. }
+          { eapply (singleton_well_ordered fts). }
+        }
+        i. des. ss. des.
+        { subst. right. eapply INJ; eauto. }
+        { left. eauto. }
+      }
+      { eapply sub_well_ordered.
+        { eapply IHl. }
+        i. des. ss. des; eauto. subst.
+        exfalso. eapply H. esplits; eauto. }
+    }
+  }
+  intros WO. eapply sub_well_ordered.
+  { eapply join_well_ordered.
+    { eapply WO. }
+    { eapply (finite_well_ordered (times loc)). }
+  }
+  { i. unfold certification_times in *. des; eauto. left.
+    esplits; eauto. }
+Qed.
+
+Lemma wf_time_evt_map times f te fte
+      (WF: wf_time_evt times te)
+      (MAP: tevent_map f fte te)
+  :
+    wf_time_evt (fun loc fts => exists ts, (<<IN: times loc ts>>) /\ (<<MAP: f loc ts fts>>)) fte.
+Proof.
+  inv MAP; ss.
+  { des. splits; eauto. }
+  { des. splits; eauto. }
+  { des. splits; eauto. }
+Qed.
 
 Definition pf_consistent_flex lang (e0:Thread.t lang)
            (tr : list (ThreadEvent.t * Memory.t)) (times : Loc.t -> list Time.t)
@@ -282,7 +363,7 @@ Definition pf_consistent_flex lang (e0:Thread.t lang)
                         (CAP: cap_flex e0.(Thread.memory) mem1 (fun loc => incr_time_seq (tm loc))),
       exists ftr e1,
         (<<STEPS: traced_step ftr (Thread.mk _ e0.(Thread.state) e0.(Thread.local) TimeMap.bot mem1) e1>>) /\
-        (<<EVENTS: List.Forall (fun em => <<SAT: (promise_free /1\ no_sc /1\ write_not_in (fun loc ts => (<<TS: Time.le ts (incr_time_seq (tm loc))>>) /\ (<<PROM: ~ covered loc ts e0.(Thread.local).(Local.promises)>>))) (fst em)>> /\ <<TAU: ThreadEvent.get_machine_event (fst em) = MachineEvent.silent>>) ftr >>) /\
+        (<<EVENTS: List.Forall (fun em => <<SAT: (promise_free /1\ no_sc /1\ write_not_in (fun loc ts => (<<TS: Time.le ts (incr_time_seq (tm loc))>>) /\ (<<PROM: ~ covered loc ts e0.(Thread.local).(Local.promises)>>)) /1\ wf_time_evt (fun loc => certification_times times f (Memory.max_timemap e0.(Thread.memory)) loc)) (fst em)>> /\ <<TAU: ThreadEvent.get_machine_event (fst em) = MachineEvent.silent>>) ftr >>) /\
         (<<TRACE: List.Forall2 (fun em fem => <<EVENT: tevent_map (fun loc => f loc (tm loc)) (fst fem) (fst em)>> /\ <<MEM: memory_map (fun loc => f loc (tm loc)) (snd em) (snd fem)>>) tr ftr>>) /\
         (__guard__((exists st',
                        (<<LOCAL: Local.failure_step e1.(Thread.local)>>) /\
@@ -381,17 +462,31 @@ Proof.
   exists ftr, (Thread.mk _ state flc1 fsc1 fmem1). splits; auto.
   { eapply List.Forall_forall. i.
     cut ((promise_free /1\ no_sc) (fst x) /\ ThreadEvent.get_machine_event (fst x) = MachineEvent.silent).
-    { i. des. splits; auto. eapply List.Forall_forall in H; eauto. ss.
-      eapply write_not_in_mon_bot; eauto. intros loc ts. intros. des.
-      assert (ITV: Interval.mem (Time.bot, incr_time_seq (tm loc)) ts).
-      { econs; ss. }
-      erewrite (@cap_flex_covered _ _ (fun loc => incr_time_seq (tm loc))) in ITV; eauto.
-      inv ITV. econs; eauto. econs; eauto.
-      destruct (Memory.get loc to (Local.promises (Thread.local th)))
-        as [[from' msg']|] eqn:GETPROM; eauto.
-      exfalso. dup GETPROM.
-      eapply WF in GETPROM. eapply CAP0 in GETPROM. clarify.
-      eapply SAT0. econs; eauto.
+    { i. des. splits; auto.
+      { eapply List.Forall_forall in H; eauto. ss.
+        eapply write_not_in_mon_bot; eauto. intros loc ts. intros. des.
+        assert (ITV: Interval.mem (Time.bot, incr_time_seq (tm loc)) ts).
+        { econs; ss. }
+        erewrite (@cap_flex_covered _ _ (fun loc => incr_time_seq (tm loc))) in ITV; eauto.
+        inv ITV. econs; eauto. econs; eauto.
+        destruct (Memory.get loc to (Local.promises (Thread.local th)))
+          as [[from' msg']|] eqn:GETPROM; eauto.
+        exfalso. dup GETPROM.
+        eapply WF in GETPROM. eapply CAP0 in GETPROM. clarify.
+        eapply SAT0. econs; eauto. }
+      { eapply list_Forall2_in in H; eauto. des.
+        eapply List.Forall_forall in IN; eauto. ss. des.
+        eapply wf_time_evt_map in SAT0; eauto. eapply wf_time_evt_mon; try apply SAT0.
+        i. ss. des. destruct (Time.le_lt_dec ts (Memory.max_timemap (Thread.memory th) x0)).
+        { left. assert (ts = x2).
+          { eapply mapping_map_lt_map_eq.
+            { eapply MAP. }
+            { ss. eapply MAP. eauto. }
+            { eauto. }
+          }
+          subst. eauto. }
+        { right. esplits; eauto. }
+      }
     }
     eapply list_Forall2_in in H; eauto. des.
     eapply List.Forall_forall in IN; eauto. ss. des.
@@ -436,7 +531,7 @@ Definition pf_consistent_flex_aux lang (e0:Thread.t lang)
                         (TM1: forall loc, Time.lt (Memory.max_ts loc mem1) (incr_time_seq (tm loc))),
       exists ftr e1,
         (<<STEPS: traced_step ftr (Thread.mk _ e0.(Thread.state) e0.(Thread.local) TimeMap.bot mem1) e1>>) /\
-        (<<EVENTS: List.Forall (fun em => <<SAT: (promise_free /1\ no_sc /1\ write_not_in (fun loc ts => (<<TS: Time.le ts (incr_time_seq (tm loc))>>) /\ (<<PROM: ~ covered loc ts e0.(Thread.local).(Local.promises)>>))) (fst em)>> /\ <<TAU: ThreadEvent.get_machine_event (fst em) = MachineEvent.silent>>) ftr >>) /\
+        (<<EVENTS: List.Forall (fun em => <<SAT: (promise_free /1\ no_sc /1\ write_not_in (fun loc ts => (<<TS: Time.le ts (incr_time_seq (tm loc))>>) /\ (<<PROM: ~ covered loc ts e0.(Thread.local).(Local.promises)>>)) /1\ wf_time_evt (fun loc => certification_times times f (Memory.max_timemap e0.(Thread.memory)) loc)) (fst em)>> /\ <<TAU: ThreadEvent.get_machine_event (fst em) = MachineEvent.silent>>) ftr >>) /\
         (<<TRACE: List.Forall2 (fun em fem => tevent_map (fun loc => f loc (tm loc)) (fst fem) (fst em)) tr ftr>>) /\
         (__guard__((exists st',
                        (<<LOCAL: Local.failure_step e1.(Thread.local)>>) /\
@@ -484,10 +579,14 @@ Proof.
   splits; auto.
   { eapply List.Forall_forall. i.
     cut ((promise_free /1\ no_sc) (fst x) /\ ThreadEvent.get_machine_event (fst x) = MachineEvent.silent).
-    { i. des. splits; auto.
-      eapply list_Forall2_in in H; eauto. des.
+    { i. des. eapply list_Forall2_in in H; eauto. des.
       eapply List.Forall_forall in IN; eauto. ss. des.
-      eapply ident_map_write_not_in; eauto. }
+      splits; auto.
+      { eapply ident_map_write_not_in; eauto. }
+      { eapply wf_time_evt_map in SAT0; eauto.
+        eapply wf_time_evt_mon; try apply SAT0. ss.
+        i. des. inv MAP0. eauto. }
+    }
     eapply list_Forall2_in in H; eauto. des.
     eapply List.Forall_forall in IN; eauto. ss. des.
     destruct x, a. ss. inv EVENT; ss. inv KIND; ss.
@@ -514,22 +613,24 @@ Proof.
 Qed.
 
 Definition pf_consistent_super_strong lang (e0:Thread.t lang)
-           (tr : list (ThreadEvent.t * Memory.t)) (times : Loc.t -> list Time.t): Prop :=
+           (tr : list (ThreadEvent.t * Memory.t))
+           (times: Loc.t -> list Time.t)
+           (certimes: Loc.t -> (Time.t -> Prop))
+  : Prop :=
   forall mem1 tm sc
          (FUTURE: Memory.future_weak e0.(Thread.memory) mem1)
          (CLOSED: Memory.closed mem1)
-         (LOCAL: Local.wf e0.(Thread.local) mem1)
-         (TM0: forall loc, Time.lt (Memory.max_ts loc e0.(Thread.memory)) (tm loc))
-         (TM1: forall loc, Time.lt (Memory.max_ts loc mem1) (tm loc)),
-  exists ftr e1 f,
+         (LOCAL: Local.wf e0.(Thread.local) mem1),
+  exists ftm ftr e1 f,
+    (<<TM: TimeMap.le tm ftm>>) /\
     (<<STEPS: traced_step ftr (Thread.mk _ e0.(Thread.state) e0.(Thread.local) sc mem1) e1>>) /\
-    (<<EVENTS: List.Forall (fun em => <<SAT: (promise_free /1\ no_sc) (fst em)>> /\ <<TAU: ThreadEvent.get_machine_event (fst em) = MachineEvent.silent>>) ftr >>) /\
+    (<<EVENTS: List.Forall (fun em => <<SAT: (promise_free /1\ no_sc /1\ wf_time_evt certimes) (fst em)>> /\ <<TAU: ThreadEvent.get_machine_event (fst em) = MachineEvent.silent>>) ftr >>) /\
     (<<MAP: cap_flex_map
               (Memory.max_timemap e0.(Thread.memory))
               (fun loc => Time.incr (Memory.max_ts loc e0.(Thread.memory)))
-              tm times f>>) /\
+              ftm times f>>) /\
     (<<TRACE: List.Forall2 (fun em fem => tevent_map f (fst fem) (fst em)) tr ftr>>) /\
-    (<<GOOD: good_future tm mem1 e1.(Thread.memory)>>) /\
+    (<<GOOD: good_future ftm mem1 e1.(Thread.memory)>>) /\
     (<<SC: e1.(Thread.sc) = sc>>) /\
     (__guard__((exists st',
                    (<<LOCAL: Local.failure_step e1.(Thread.local)>>) /\
@@ -541,28 +642,60 @@ Definition pf_consistent_super_strong lang (e0:Thread.t lang)
                       (<<WRITING: promise_writing_event loc from to val released e>>) /\
                       (<<IN: List.In (e, m) ftr>>)>>)))).
 
-
-wf_time_evt
-
-mappable_evt
-
-Lemma pf_consistent_flex_aux_pf_consistent_super_strong lang (th: Thread.t lang) tr times
+Lemma pf_consistent_flex_aux_pf_consistent_super_strong lang (th: Thread.t lang) tr times f
       (WF: Local.wf th.(Thread.local) th.(Thread.memory))
       (MEM: Memory.closed th.(Thread.memory))
-      (CONSISTENT: pf_consistent_flex_aux th tr times)
+      (CONSISTENT: pf_consistent_flex_aux th tr times f)
   :
-    pf_consistent_super_strong th tr times.
+    exists certimes,
+      (<<WO: forall loc, well_ordered (certimes loc)>>) /\
+      (<<CONSISTENT: pf_consistent_super_strong th tr times certimes>>).
 Proof.
-  ii. exploit CONSISTENT; eauto. i. des. destruct e1.
+  unfold pf_consistent_flex_aux in *. des.
+  exists (certification_times times f (Memory.max_timemap th.(Thread.memory))). splits.
+  { eapply certification_times_well_ordered. eauto. }
+  ii. assert (TM: exists (ftm: Loc.t -> nat),
+                 forall loc,
+                   (<<TM0: Time.lt (Memory.max_ts loc th.(Thread.memory)) (incr_time_seq (ftm loc))>>) /\
+                   (<<TM1: Time.lt (Memory.max_ts loc mem1) (incr_time_seq (ftm loc))>>) /\
+                   (<<TM2: Time.le (tm loc) (incr_time_seq (ftm loc))>>)).
+  { eapply (choice
+              (fun loc n =>
+                 (<<TM0: Time.lt (Memory.max_ts loc th.(Thread.memory)) (incr_time_seq n)>>) /\
+                 (<<TM1: Time.lt (Memory.max_ts loc mem1) (incr_time_seq n)>>) /\
+                 (<<TM2: Time.le (tm loc) (incr_time_seq n)>>))).
+    intros loc. hexploit (incr_time_seq_diverge
+                            (Time.join (Time.join
+                                          (Memory.max_ts loc th.(Thread.memory))
+                                          (Memory.max_ts loc mem1))
+                                       (tm loc))).
+    i. des. exists n. splits.
+    { eapply TimeFacts.le_lt_lt; eauto. etrans.
+      { eapply Time.join_l. }
+      eapply Time.join_l. }
+    { eapply TimeFacts.le_lt_lt; eauto. etrans.
+      { eapply Time.join_r. }
+      eapply Time.join_l. }
+    { left. eapply TimeFacts.le_lt_lt; eauto.
+      eapply Time.join_r. }
+  }
+  des. hexploit (CONSISTENT0 mem1 ftm); eauto.
+  { eapply TM; eauto. }
+  { eapply TM; eauto. }
+  i. des. destruct e1.
   exploit write_not_in_good_future_traced; try apply STEPS; ss; auto.
+  { eapply TM. }
   { eapply Memory.closed_timemap_bot. inv CLOSED. auto. }
   { eapply List.Forall_impl; eauto. i. ss. des. eapply write_not_in_mon; eauto.
     i. ss. des. split; auto. ii. eapply PROM.
-    inv H. econs; eauto. eapply LOCAL in GET; eauto. }
+    inv H. econs; eauto. eapply LOCAL in GET; eauto. } intros GOOD.
   eapply no_sc_any_sc_traced in STEPS; ss; cycle 1.
   { i. eapply List.Forall_forall in IN; eauto. ss. des; auto. } des.
+  eexists (fun loc => incr_time_seq (ftm loc)), ftr, _, (fun loc => f loc (ftm loc)).
   esplits; eauto.
+  { ii. eapply TM. }
   { eapply List.Forall_impl; [|apply EVENTS]. i. ss. des; auto. }
+  { eapply cap_flex_map_locwise. i. eapply MAP. eapply TM. }
   { eapply no_sc_same_sc_traced in STEPS0; eauto.
     eapply List.Forall_impl; eauto. i. ss. des; auto. }
 Qed.
@@ -572,291 +705,9 @@ Lemma consistent_pf_consistent_super_strong lang (th: Thread.t lang)
       (MEM: Memory.closed th.(Thread.memory))
       (CONSISTENT: Thread.consistent th)
   :
-    exists tr times, <<CONSISTENT: pf_consistent_super_strong th tr times>>.
-Proof.
-  eapply consistent_pf_consistent in CONSISTENT; eauto.
-  eapply pf_consistent_pf_consistent_strong in CONSISTENT; eauto.
-  eapply pf_consistent_strong_pf_consistent_strong_aux in CONSISTENT; eauto.
-  eapply pf_consistent_strong_aux_pf_consistent_flex in CONSISTENT; eauto. des.
-  eapply pf_consistent_flex_pf_consistent_flex_aux in CONSISTENT0; eauto.
-  eapply pf_consistent_flex_aux_pf_consistent_super_strong in CONSISTENT0; eauto.
-Qed.
-
-
-
-
-
-
-Definition pf_consistent_flex lang (e0:Thread.t lang)
-           (tr : list (ThreadEvent.t * Memory.t)) (times : Loc.t -> list Time.t): Prop :=
-  forall mem1 tm
-         (TM: forall loc, Time.lt (Memory.max_ts loc e0.(Thread.memory)) (tm loc))
-         (CAP: cap_flex e0.(Thread.memory) mem1 tm),
-  exists ftr e1 f,
-    (<<STEPS: traced_step ftr (Thread.mk _ e0.(Thread.state) e0.(Thread.local) TimeMap.bot mem1) e1>>) /\
-    (<<EVENTS: List.Forall (fun em => <<SAT: (promise_free /1\ no_sc /1\ write_not_in (fun loc ts => (<<TS: Time.le ts (tm loc)>>) /\ (<<PROM: ~ covered loc ts e0.(Thread.local).(Local.promises)>>))) (fst em)>> /\ <<TAU: ThreadEvent.get_machine_event (fst em) = MachineEvent.silent>>) ftr >>) /\
-    (<<MAP: cap_flex_map
-              (Memory.max_timemap e0.(Thread.memory))
-              (fun loc => Time.incr (Memory.max_ts loc e0.(Thread.memory)))
-              tm times f>>) /\
-    (<<TRACE: List.Forall2 (fun em fem => <<EVENT: tevent_map f (fst fem) (fst em)>> /\ <<MEM: memory_map f (snd em) (snd fem)>>) tr ftr>>) /\
-    (__guard__((exists st',
-                   (<<LOCAL: Local.failure_step e1.(Thread.local)>>) /\
-                   (<<FAILURE: Language.step lang ProgramEvent.failure (@Thread.state lang e1) st'>>)) \/
-               ((<<PROMISES: e1.(Thread.local).(Local.promises) = Memory.bot>>) /\
-                (<<WRITES: forall loc from to val released
-                                  (GET: Memory.get loc to e0.(Thread.local).(Local.promises) = Some (from, Message.concrete val released)),
-                    exists e m,
-                      (<<WRITING: promise_writing_event loc from to val released e>>) /\
-                      (<<IN: List.In (e, m) ftr>>)>>)))).
-
-Lemma pf_consistent_strong_aux_pf_consistent_flex lang (th: Thread.t lang)
-      (WF: Local.wf th.(Thread.local) th.(Thread.memory))
-      (MEM: Memory.closed th.(Thread.memory))
-      (CONSISTENT: pf_consistent_strong_aux th)
-  :
-    exists tr times, <<CONSISTENT: pf_consistent_flex th tr times>>.
-Proof.
-  exploit Memory.cap_exists; eauto. i. des.
-  exploit CONSISTENT; eauto. i. des.
-  exists tr, times. ii.
-  exploit (@cap_flex_map_exists
-             (Memory.max_timemap th.(Thread.memory))
-             (fun loc => Time.incr (Memory.max_ts loc th.(Thread.memory)))
-             tm).
-  { i. eapply Time.incr_spec. }
-  { auto. }
-  i. des. destruct e1. ss.
-  hexploit traced_steps_map.
-  { eapply mapping_map_lt_map_le. eapply MAP. }
-  { eapply MAP. }
-  { eapply mapping_map_lt_map_eq. eapply MAP. }
-  { eapply wf_time_mapped_mappable.
-    { eapply List.Forall_impl; eauto. i. ss. des; eauto. }
-    { eapply cap_flex_map_complete; eauto. }
-  }
-  { eapply STEPS. }
-  { ss. }
-  { ss. }
-  { ss. }
-  { eapply Local.cap_wf; eauto. }
-  { instantiate (1:=mem1). instantiate (1:=th.(Thread.local)).
-    eapply cap_flex_wf; eauto. }
-  { eapply cap_flex_closed; eauto. }
-  { eapply Memory.cap_closed; eauto. }
-  { eapply Memory.closed_timemap_bot.
-    eapply cap_flex_closed in CAP0; auto. eapply CAP0. }
-  { eapply Memory.closed_timemap_bot.
-    eapply Memory.cap_closed in CAP; auto. eapply CAP. }
-  { eapply map_ident_in_memory_local.
-    { ii. eapply MAP. eapply TS. }
-    { eapply MAP. }
-    { eauto. }
-    { eauto. }
-  }
-  { eapply concrete_messages_le_cap_flex_memory_map.
-    { refl. }
-    { instantiate (1:=(fun loc => Time.incr (Memory.max_ts loc th.(Thread.memory)))).
-      i. eapply Time.incr_spec. }
-    { eapply TM. }
-    { eapply cap_cap_flex; eauto. }
-    { eauto. }
-    { eauto. }
-    { eauto. }
-    { eauto. }
-  }
-  { eapply mapping_map_lt_collapsable_unwritable. eapply MAP. }
-  { eapply timemap_bot_map. eapply MAP. }
-  { refl. } i. des.
-  exploit write_not_in_traced; eauto.
-  { ss. transitivity (th.(Thread.memory)).
-    { eapply WF. }
-    { eapply CAP0. }
-  } intros NOTIN. ss.
-  exists ftr, (Thread.mk _ state flc1 fsc1 fmem1), f. splits; auto.
-  { eapply List.Forall_forall. i.
-    cut ((promise_free /1\ no_sc) (fst x) /\ ThreadEvent.get_machine_event (fst x) = MachineEvent.silent).
-    { i. des. splits; auto. eapply List.Forall_forall in H; eauto. ss.
-      eapply write_not_in_mon_bot; eauto. intros loc ts. intros. des.
-      assert (ITV: Interval.mem (Time.bot, tm loc) ts).
-      { econs; ss. }
-      erewrite cap_flex_covered in ITV; eauto.
-      inv ITV. econs; eauto. econs; eauto.
-      destruct (Memory.get loc to (Local.promises (Thread.local th)))
-        as [[from' msg']|] eqn:GETPROM; eauto.
-      exfalso. dup GETPROM.
-      eapply WF in GETPROM. eapply CAP0 in GETPROM. clarify.
-      eapply SAT0. econs; eauto.
-    }
-    eapply list_Forall2_in in H; eauto. des.
-    eapply List.Forall_forall in IN; eauto. ss. des.
-    destruct x, a. ss. inv EVENT; ss. inv KIND; ss.
-    splits; auto. inv MSG0; ss. inv MSG; ss. inv MAP1; ss.
-  }
-  { ss. unguard. des; eauto.
-    { left. esplits; eauto. eapply failure_step_map; eauto.
-      { eapply mapping_map_lt_map_le. eapply MAP. }
-      { eapply mapping_map_lt_map_eq. eapply MAP. }
-    }
-    { right. splits.
-      { inv LOCAL. erewrite PROMISES in *. eapply bot_promises_map; eauto. }
-      { i. exploit WRITES; eauto. i. des.
-        eapply list_Forall2_in2 in IN; eauto. des.
-        destruct b. ss. eexists t, _. splits; eauto.
-        eapply promise_writing_event_map; eauto.
-        { inv WF. eapply PROMISES0 in GET. eauto. }
-        { eapply MAP. }
-        { ii. eapply MAP. auto. }
-      }
-    }
-  }
-Qed.
-
-Definition pf_consistent_flex_aux lang (e0:Thread.t lang)
-           (tr : list (ThreadEvent.t * Memory.t)) (times : Loc.t -> list Time.t): Prop :=
-  forall mem1 tm
-         (FUTURE: Memory.future_weak e0.(Thread.memory) mem1)
-         (CLOSED: Memory.closed mem1)
-         (LOCAL: Local.wf e0.(Thread.local) mem1)
-         (TM0: forall loc, Time.lt (Memory.max_ts loc e0.(Thread.memory)) (tm loc))
-         (TM1: forall loc, Time.lt (Memory.max_ts loc mem1) (tm loc)),
-  exists ftr e1 f,
-    (<<STEPS: traced_step ftr (Thread.mk _ e0.(Thread.state) e0.(Thread.local) TimeMap.bot mem1) e1>>) /\
-    (<<EVENTS: List.Forall (fun em => <<SAT: (promise_free /1\ no_sc /1\ write_not_in (fun loc ts => (<<TS: Time.le ts (tm loc)>>) /\ (<<PROM: ~ covered loc ts e0.(Thread.local).(Local.promises)>>))) (fst em)>> /\ <<TAU: ThreadEvent.get_machine_event (fst em) = MachineEvent.silent>>) ftr >>) /\
-    (<<MAP: cap_flex_map
-              (Memory.max_timemap e0.(Thread.memory))
-              (fun loc => Time.incr (Memory.max_ts loc e0.(Thread.memory)))
-              tm times f>>) /\
-    (<<TRACE: List.Forall2 (fun em fem => tevent_map f (fst fem) (fst em)) tr ftr>>) /\
-    (__guard__((exists st',
-                   (<<LOCAL: Local.failure_step e1.(Thread.local)>>) /\
-                   (<<FAILURE: Language.step lang ProgramEvent.failure (@Thread.state lang e1) st'>>)) \/
-               ((<<PROMISES: e1.(Thread.local).(Local.promises) = Memory.bot>>) /\
-                (<<WRITES: forall loc from to val released
-                                  (GET: Memory.get loc to e0.(Thread.local).(Local.promises) = Some (from, Message.concrete val released)),
-                    exists e m,
-                      (<<WRITING: promise_writing_event loc from to val released e>>) /\
-                      (<<IN: List.In (e, m) ftr>>)>>)))).
-
-Lemma pf_consistent_flex_pf_consistent_flex_aux lang (th: Thread.t lang) tr times
-      (WF: Local.wf th.(Thread.local) th.(Thread.memory))
-      (MEM: Memory.closed th.(Thread.memory))
-      (CONSISTENT: pf_consistent_flex th tr times)
-  :
-    pf_consistent_flex_aux th tr times.
-Proof.
-  ii. exploit (@cap_flex_exists th.(Thread.memory) tm); eauto. i. des.
-  exploit CONSISTENT; eauto. i. des. destruct e1. ss.
-  hexploit traced_steps_map.
-  { eapply ident_map_le; eauto. }
-  { eapply ident_map_bot; eauto. }
-  { eapply ident_map_eq; eauto. }
-  { eapply List.Forall_forall. i. eapply ident_map_mappable_evt. }
-  { eapply STEPS. }
-  { ss. }
-  { ss. }
-  { ss. }
-  { eapply cap_flex_wf; eauto. }
-  { eapply LOCAL. }
-  { eauto. }
-  { eapply cap_flex_closed; eauto. }
-  { eapply Memory.closed_timemap_bot. inv CLOSED. auto. }
-  { eapply Memory.closed_timemap_bot.
-    eapply cap_flex_closed in CAP; eauto. eapply CAP. }
-  { eapply ident_map_local. }
-  { eapply cap_flex_future_memory_map; try apply CAP; eauto.
-    ii. left. eauto. }
-  { eapply mapping_map_lt_collapsable_unwritable. eapply ident_map_lt. }
-  { eapply timemap_bot_map. eapply ident_map_bot. }
-  { refl. }
-  i. des. exists ftr0, (Thread.mk _ state flc1 fsc1 fmem1), f.
-  splits; auto.
-  { eapply List.Forall_forall. i.
-    cut ((promise_free /1\ no_sc) (fst x) /\ ThreadEvent.get_machine_event (fst x) = MachineEvent.silent).
-    { i. des. splits; auto.
-      eapply list_Forall2_in in H; eauto. des.
-      eapply List.Forall_forall in IN; eauto. ss. des.
-      eapply ident_map_write_not_in; eauto. }
-    eapply list_Forall2_in in H; eauto. des.
-    eapply List.Forall_forall in IN; eauto. ss. des.
-    destruct x, a. ss. inv EVENT; ss. inv KIND; ss.
-    splits; auto. inv MSG0; ss. inv MSG; ss. inv MAP1; ss. }
-    { eapply list_Forall2_compose; eauto.
-    i. ss. des. eapply ident_map_compose_tevent; eauto. }
-  { ss. unguard. des; eauto.
-    { left. esplits; eauto. eapply failure_step_map; eauto.
-      { eapply ident_map_le. }
-      { eapply ident_map_eq. }
-    }
-    { right. splits.
-      { inv LOCAL0. erewrite PROMISES in *. eapply bot_promises_map; eauto. }
-      { i. exploit WRITES; eauto. i. des.
-        eapply list_Forall2_in2 in IN; eauto. des.
-        destruct b. ss. eexists t, _. splits; eauto.
-        eapply promise_writing_event_map; eauto.
-        { inv LOCAL. eapply PROMISES0 in GET. eauto. }
-        { eapply ident_map_lt. }
-        { ii. ss. }
-      }
-    }
-  }
-Qed.
-
-Definition pf_consistent_super_strong lang (e0:Thread.t lang)
-           (tr : list (ThreadEvent.t * Memory.t)) (times : Loc.t -> list Time.t): Prop :=
-  forall mem1 tm sc
-         (FUTURE: Memory.future_weak e0.(Thread.memory) mem1)
-         (CLOSED: Memory.closed mem1)
-         (LOCAL: Local.wf e0.(Thread.local) mem1)
-         (TM0: forall loc, Time.lt (Memory.max_ts loc e0.(Thread.memory)) (tm loc))
-         (TM1: forall loc, Time.lt (Memory.max_ts loc mem1) (tm loc)),
-  exists ftr e1 f,
-    (<<STEPS: traced_step ftr (Thread.mk _ e0.(Thread.state) e0.(Thread.local) sc mem1) e1>>) /\
-    (<<EVENTS: List.Forall (fun em => <<SAT: (promise_free /1\ no_sc) (fst em)>> /\ <<TAU: ThreadEvent.get_machine_event (fst em) = MachineEvent.silent>>) ftr >>) /\
-    (<<MAP: cap_flex_map
-              (Memory.max_timemap e0.(Thread.memory))
-              (fun loc => Time.incr (Memory.max_ts loc e0.(Thread.memory)))
-              tm times f>>) /\
-    (<<TRACE: List.Forall2 (fun em fem => tevent_map f (fst fem) (fst em)) tr ftr>>) /\
-    (<<GOOD: good_future tm mem1 e1.(Thread.memory)>>) /\
-    (<<SC: e1.(Thread.sc) = sc>>) /\
-    (__guard__((exists st',
-                   (<<LOCAL: Local.failure_step e1.(Thread.local)>>) /\
-                   (<<FAILURE: Language.step lang ProgramEvent.failure (@Thread.state lang e1) st'>>)) \/
-               ((<<PROMISES: e1.(Thread.local).(Local.promises) = Memory.bot>>) /\
-                (<<WRITES: forall loc from to val released
-                                  (GET: Memory.get loc to e0.(Thread.local).(Local.promises) = Some (from, Message.concrete val released)),
-                    exists e m,
-                      (<<WRITING: promise_writing_event loc from to val released e>>) /\
-                      (<<IN: List.In (e, m) ftr>>)>>)))).
-
-Lemma pf_consistent_flex_aux_pf_consistent_super_strong lang (th: Thread.t lang) tr times
-      (WF: Local.wf th.(Thread.local) th.(Thread.memory))
-      (MEM: Memory.closed th.(Thread.memory))
-      (CONSISTENT: pf_consistent_flex_aux th tr times)
-  :
-    pf_consistent_super_strong th tr times.
-Proof.
-  ii. exploit CONSISTENT; eauto. i. des. destruct e1.
-  exploit write_not_in_good_future_traced; try apply STEPS; ss; auto.
-  { eapply Memory.closed_timemap_bot. inv CLOSED. auto. }
-  { eapply List.Forall_impl; eauto. i. ss. des. eapply write_not_in_mon; eauto.
-    i. ss. des. split; auto. ii. eapply PROM.
-    inv H. econs; eauto. eapply LOCAL in GET; eauto. }
-  eapply no_sc_any_sc_traced in STEPS; ss; cycle 1.
-  { i. eapply List.Forall_forall in IN; eauto. ss. des; auto. } des.
-  esplits; eauto.
-  { eapply List.Forall_impl; [|apply EVENTS]. i. ss. des; auto. }
-  { eapply no_sc_same_sc_traced in STEPS0; eauto.
-    eapply List.Forall_impl; eauto. i. ss. des; auto. }
-Qed.
-
-Lemma consistent_pf_consistent_super_strong lang (th: Thread.t lang)
-      (LOCAL: Local.wf th.(Thread.local) th.(Thread.memory))
-      (MEM: Memory.closed th.(Thread.memory))
-      (CONSISTENT: Thread.consistent th)
-  :
-    exists tr times, <<CONSISTENT: pf_consistent_super_strong th tr times>>.
+    exists tr times certimes,
+      (<<WO: forall loc, well_ordered (certimes loc)>>) /\
+      <<CONSISTENT: pf_consistent_super_strong th tr times certimes>>.
 Proof.
   eapply consistent_pf_consistent in CONSISTENT; eauto.
   eapply pf_consistent_pf_consistent_strong in CONSISTENT; eauto.
